wip on adapting compiler

compiler/src/FlatToRiscvBitWidthSpecifics.v
@@ -1,41 +1,8 @@
+Require Import coqutil.Map.Interface.
 Require Import riscv.util.BitWidths.
 Require Import riscv.Utility.
 Require Import riscv.Memory.
 
-Class FlatToRiscvBitWidthSpecifics(mword: Set){MW: MachineWidth mword}{MF: MemoryFunctions mword} := {
+Class FlatToRiscvBitWidthSpecifics(mword: Type){MW: MachineWidth mword}{Mem: map.map mword byte} := {
   BitWidth: BitWidths;
-
-  loadWordwXLEN: Mem mword -> mword ->  mword;
-
-  storeWordwXLEN: Mem mword -> mword -> mword -> Mem mword;
-
 }.
-
-(*
-  Definition loadWordwXLEN(memL: mem)(addr: mword): mword.
-    clear -addr memL IsMem B mword_word_wXLEN.
-    rewrite mword_word_wXLEN.
-    unfold wXLEN in *.
-    destruct bitwidth.
-    - exact (Memory.loadWord memL addr).
-    - exact (Memory.loadDouble memL addr).
-  Defined.
-
-  Definition TODO{T: Type}: T. Proof using. Admitted.
-
-  Definition storeWordwXLEN(m: mem)(a v: mword): mem.
-    unfold wXLEN, bitwidth in *.
-    clear - m a v IsMem mword_word_wXLEN.
-    rewrite mword_word_wXLEN in *.
-    destruct B.
-    - refine (Memory.storeWord m a v).
-      Fail rewrite mword_word_wXLEN in IsMem.
-      apply TODO.
-    - refine (Memory.storeDouble m a v). apply TODO.
-      Grab Existential Variables.
-      apply TODO. apply TODO.
-  Defined.
-
-
-  BitWidths.BitWidths
-*)
