compiler/src/FlatToRiscv32Specifics.v
@@ -1,19 +1,16 @@
+Require Import coqutil.Map.Interface.
 Require Import riscv.util.Word.
 Require Import riscv.util.BitWidths.
+Require Import riscv.MachineWidth32.
 Require Import riscv.Utility.
 Require Import compiler.FlatToRiscvBitWidthSpecifics.
 Require Import riscv.Memory.
 
 
-Instance FlatToRiscv32Specifics{MW: MachineWidth (word 32)}{MF: MemoryFunctions (word 32)}
-  : FlatToRiscvBitWidthSpecifics (word 32)  := {|
+Instance FlatToRiscv32Specifics{Mem: map.map word32 byte}
+  : FlatToRiscvBitWidthSpecifics word32  := {|
 
   BitWidth := BW32;
-
-  loadWordwXLEN := loadWord;
-
-  storeWordwXLEN := storeWord;
-
 |}.
 
 (* old compile_lit code, TODO reactivate
