compiler/src/FlatToRiscv64Specifics.v
@@ -1,16 +1,13 @@
+Require Import coqutil.Map.Interface.
 Require Import riscv.util.Word.
 Require Import riscv.util.BitWidths.
+Require Import riscv.MachineWidth64.
 Require Import riscv.Utility.
 Require Import compiler.FlatToRiscvBitWidthSpecifics.
 Require Import riscv.Memory.
 
-
-Instance FlatToRiscv64Specifics{MW: MachineWidth (word 64)}{MF: MemoryFunctions (word 64)}
-  : FlatToRiscvBitWidthSpecifics (word 64)  := {|
+Instance FlatToRiscv64Specifics{Mem: map.map word64 byte}
+  : FlatToRiscvBitWidthSpecifics word64  := {|
 
   BitWidth := BW64;
-
-  loadWordwXLEN := loadDouble;
-
-  storeWordwXLEN := storeDouble;
 |}.
